Tweak the value relation. Proofs need fixing.
Previously it related closures by applying them to exactly the number of
arguments needed to make them actually run. That was simple, but too
weak, because you then know nothing about related closures applied to
too few arguments.

compiler1/semantics/closRelationScript.sml
@@ -75,6 +75,11 @@ val clo_to_loc_def = Define `
 (clo_to_loc (Closure l _ _ _ _) = l) ∧
 (clo_to_loc (Recclosure l _ _ _ i) = OPTION_MAP ((+) i) l)`;
 
+val clo_to_env_def = Define `
+(clo_to_env (Closure _ _ env _ _) = env) ∧
+(clo_to_env (Recclosure loc _ env fns _) = 
+  GENLIST (Recclosure loc [] env fns) (LENGTH fns) ++ env)`;
+
 val clo_to_partial_args_def = Define `
 (clo_to_partial_args (Closure _ args _ _ _) = args) ∧
 (clo_to_partial_args (Recclosure _ args _ _ _) = args)`;
@@ -112,7 +117,8 @@ val val_rel_def = tDefine "val_rel" `
     !i' args args' s s'.
       if i' < i then
         state_rel i' s s' ∧
-        LENGTH args = clo_to_num_params cl - LENGTH (clo_to_partial_args cl) ∧
+        args ≠ [] ∧
+        (*LENGTH args = clo_to_num_params cl - LENGTH (clo_to_partial_args cl) ∧*)
         LIST_REL (val_rel i') args args'
         ⇒
         exec_cl_rel i' (cl, args, s) (cl', args', s')
@@ -361,7 +367,8 @@ val val_rel_cl_rw = Q.store_thm ("val_rel_cl_rw",
         i' < c
         ⇒
         state_rel i' s s' ∧
-        LENGTH args = clo_to_num_params v - LENGTH (clo_to_partial_args v) ∧
+        args ≠ [] ∧
+        (* LENGTH args = clo_to_num_params v - LENGTH (clo_to_partial_args v) ∧*)
         LIST_REL (val_rel i') args args'
         ⇒
         exec_cl_rel i' (v, args, s) (v', args', s')
@@ -525,6 +532,24 @@ val dest_closure_opt = Q.store_thm ("dest_closure_opt",
      fs [OPTION_MAP_DEF] >>
      metis_tac [NOT_SOME_NONE, LENGTH_EQ_NUM, NOT_LESS_EQUAL]));
 
+val dest_closure_full_length = Q.store_thm ("dest_closure_full_length",
+`!l v vs e args rest.
+  dest_closure l v vs = SOME (Full_app e args rest)
+  ⇒
+  LENGTH vs + LENGTH (clo_to_partial_args v) = clo_to_num_params v + LENGTH rest ∧
+  LENGTH args = clo_to_num_params v + LENGTH (clo_to_env v)`,
+ rpt gen_tac >>
+ simp [dest_closure_def] >>
+ BasicProvers.EVERY_CASE_TAC >>
+ fs [is_closure_def, clo_to_partial_args_def, clo_to_num_params_def, clo_to_env_def]
+ >- (`n - LENGTH l' ≤ LENGTH vs` by decide_tac >>
+     rw [] >>
+     simp [LENGTH_TAKE]) >>
+ Cases_on `EL n l1` >>
+ fs [] >>
+ rw [] >>
+ simp []);
+
 val res_rel_evaluate_app = Q.store_thm ("res_rel_evaluate_app",
 `!c v v' vs vs' s s' loc.
   val_rel c v v' ∧
@@ -535,7 +560,9 @@ val res_rel_evaluate_app = Q.store_thm ("res_rel_evaluate_app",
   s'.clock = c
   ⇒
   res_rel (evaluate_app loc v vs s) (evaluate_app loc v' vs' s')`, 
+  cheat);
 
+  (*
  rw [] >>
  `vs' ≠ []` by (Cases_on `vs'` >> fs []) >>
  rw [evaluate_app_rw] >>
@@ -549,9 +576,19 @@ val res_rel_evaluate_app = Q.store_thm ("res_rel_evaluate_app",
  `?x'. dest_closure loc v' vs' = SOME x'` by metis_tac [dest_closure_opt] >>
  simp [] >>
  qabbrev_tac `full_arg_num = clo_to_num_params v - LENGTH (clo_to_partial_args v)` >>
- qabbrev_tac `full_arg_num' = clo_to_num_params v' - LENGTH (clo_to_partial_args v')` >>
+ Cases_on `LENGTH vs < full_arg_num` 
+ >- ((* A partial application on the left *)
+     reverse (Cases_on `x`) >>
+     fs [] 
+     >- (imp_res_tac dest_closure_full_length >>
+         full_simp_tac (srw_ss()++ARITH_ss) [Abbr `full_arg_num`]) >>
+     rw [res_rel_rw]
+     >- ((* Timeout *)
+
+
  Cases_on `x` >>
  fs []
+
  >> cheat);
  (*
  >- ((* Partial app *)
@@ -560,6 +597,7 @@ val res_rel_evaluate_app = Q.store_thm ("res_rel_evaluate_app",
          Cases_on `x'` >>
          fs []
          >- metis_tac [val_rel_mono, ZERO_LESS_EQ]     
+         *)
          *)
 
 val state_rel_refs = Q.prove (
@@ -1053,7 +1091,6 @@ val compat_app = Q.store_thm ("compat_app",
   exp_rel es es'
   ⇒
   exp_rel [App loc e es] [App loc e' es']`,
-
  rw [exp_rel_def] >>
  simp [exec_rel_rw, evaluate_def] >>
  Cases_on `LENGTH es > 0` >>
